proof/agp32_MEM_CorrectScript.sml
@@ -962,6 +962,28 @@ Proof
     by fs [Abbr `s`,agp32_MEM_isAcc_others_F] >> fs []
 QED
 
+(** do_interrupt **)
+Theorem agp32_do_interrupt_WB_enable:
+  !fext fbits a t I.
+    is_mem fext_accessor_circuit (agp32 fext fbits) fext ==>
+    enable_stg 5 (agp32 fext fbits t) ==>
+    (agp32 fext fbits (SUC t)).WB.WB_opc = 12w ==>
+    (agp32 fext fbits (SUC t)).do_interrupt
+Proof
+  rw [] >> Q.ABBREV_TAC `s = agp32 fext fbits t` >>
+  `(agp32 fext fbits (SUC t)).do_interrupt = (agp32_next_state (fext t) s s).do_interrupt`
+    by fs [agp32_interrupt_items_updated_by_agp32_next_state] >>
+  `(fext t).error = 0w` by fs [is_mem_def,mem_no_errors_def] >>     
+  `s.MEM.MEM_opc = 12w` by gs [agp32_WB_opc_MEM_opc_when_WB_enabled,Abbr `s`] >>
+  `s.MEM.MEM_isInterrupt` by gs [Abbr `s`,agp32_MEM_isInterrupt_MEM_opc_12w] >>
+  `s.state = 0w`
+    by (fs [Abbr `s`,enable_stg_def] >> Cases_on_word_value `(agp32 fext fbits t).state` >>
+        METIS_TAC [agp32_WB_state_flag_and_state,agp32_state_impossible_values]) >>     
+  `(fext t).ready`
+    by (fs [Abbr `s`,enable_stg_def] >> METIS_TAC [agp32_WB_state_flag_and_fext_ready]) >>
+  fs [agp32_next_state_def]
+QED
+
 
 (* MEM_req_rel *)
 Theorem agp32_Rel_ag32_MEM_req_rel_correct:
@@ -981,7 +1003,8 @@ Proof
       agp32_Rel_ag32_data_wdata_correct_write_mem_byte_word_bit_1,
       agp32_Rel_ag32_data_wdata_correct_write_mem_byte_word_bit_2,
       agp32_Rel_ag32_data_wdata_correct_write_mem_byte_word_bit_3,
-      agp32_Rel_ag32_acc_arg_correct,agp32_acc_arg_ready_WB_enable]
+      agp32_Rel_ag32_acc_arg_correct,agp32_acc_arg_ready_WB_enable,
+      agp32_do_interrupt_WB_enable]
 QED
 
 
